Finish typeOf_preserves_valid_refs (for real)
Signed-off-by: Zhengyao Lin <zyal@amazon.com>

cedar-lean/Cedar/Thm/SymCC/ValidRefs.lean
@@ -24,13 +24,78 @@ namespace Cedar.Thm
 
 open Spec SymCC Validation Data
 
-mutual
+/-- Shorthand form of inductive hypotheses used in the following proofs. -/
+abbrev typeOf_preserves_valid_refs_ih (Γ : TypeEnv) (entities : Entities) (e : Expr) : Prop
+:= ∀ {tx c c'},
+  typeOf e c Γ = Except.ok (tx, c') →
+  Expr.ValidRefs (fun uid => Map.contains entities uid = true) e →
+  Expr.ValidRefs (fun uid => Map.contains entities uid = true) tx.toExpr
+
+theorem typeOf_preserves_valid_refs_lit
+  {Γ : TypeEnv} (entities : Entities)
+  {p : Prim} {tx : TypedExpr} {c₁ c₂ : Capabilities}
+  (hty : typeOf (Expr.lit p) c₁ Γ = Except.ok (tx, c₂))
+  (hrefs : entities.ValidRefsFor (Expr.lit p)) :
+  entities.ValidRefsFor tx.toExpr
+:= by
+  simp only [typeOf, typeOfLit] at hty
+  cases p with
+  | bool | int | string =>
+    split at hty
+    any_goals contradiction
+    all_goals
+      simp only [
+        ok, List.empty_eq,
+        Function.comp_apply,
+        Except.ok.injEq,
+        Prod.mk.injEq,
+        List.nil_eq,
+      ] at hty
+      simp only [←hty.1, TypedExpr.toExpr]
+      repeat constructor
+  | entityUID uid =>
+    split at hty
+    any_goals contradiction
+    all_goals
+      split at hty
+      · simp only [
+          ok, List.empty_eq,
+          Function.comp_apply,
+          Except.ok.injEq,
+          Prod.mk.injEq,
+          List.nil_eq,
+        ] at hty
+        simp only [←hty.1, TypedExpr.toExpr]
+        constructor
+        cases hrefs
+        assumption
+      · contradiction
+
+theorem typeOf_preserves_valid_refs_var
+  {Γ : TypeEnv} (entities : Entities)
+  {var : Var} {tx : TypedExpr} {c₁ c₂ : Capabilities}
+  (hty : typeOf (Expr.var var) c₁ Γ = Except.ok (tx, c₂))
+  (hrefs : entities.ValidRefsFor (Expr.var var)) :
+  entities.ValidRefsFor tx.toExpr
+:= by
+  simp only [typeOf, typeOfVar] at hty
+  split at hty
+  all_goals
+    simp only [
+      ok, List.empty_eq, Function.comp_apply,
+      Except.ok.injEq, Prod.mk.injEq,
+      List.nil_eq,
+    ] at hty
+    simp only [←hty.1, TypedExpr.toExpr]
+    constructor
 
 theorem typeOf_preserves_valid_refs_and
   {Γ : TypeEnv} (entities : Entities)
   {e₁ e₂ : Expr} {tx : TypedExpr} {c₁ c₂ : Capabilities}
   (hty : typeOf (Expr.and e₁ e₂) c₁ Γ = Except.ok (tx, c₂))
-  (hrefs : entities.ValidRefsFor (Expr.and e₁ e₂)) :
+  (hrefs : entities.ValidRefsFor (Expr.and e₁ e₂))
+  (ih₁ : typeOf_preserves_valid_refs_ih Γ entities e₁)
+  (ih₂ : typeOf_preserves_valid_refs_ih Γ entities e₂) :
   entities.ValidRefsFor tx.toExpr
 := by
   cases hrefs with | and_valid hrefs₁ hrefs₂ =>
@@ -44,7 +109,7 @@ theorem typeOf_preserves_valid_refs_and
     any_goals contradiction
     · simp only [ok, Except.ok.injEq, Prod.mk.injEq, List.nil_eq] at hty
       simp only [←hty.1, TypedExpr.toExpr]
-      exact typeOf_preserves_valid_refs entities hty₁ hrefs₁
+      exact ih₁ hty₁ hrefs₁
     · cases hty₂ : typeOf e₂ (c₁ ∪ c₃) Γ with
       | error => simp [hty₂] at hty
       | ok r₂ =>
@@ -56,16 +121,16 @@ theorem typeOf_preserves_valid_refs_and
           simp only [ok, Except.ok.injEq, Prod.mk.injEq, List.nil_eq] at hty
           simp only [←hty.1, TypedExpr.toExpr]
           constructor
-          · exact typeOf_preserves_valid_refs entities hty₁ hrefs₁
-          · exact typeOf_preserves_valid_refs entities hty₂ hrefs₂
-termination_by 1 + sizeOf e₁ + sizeOf e₂
-decreasing_by all_goals sorry
+          · exact ih₁ hty₁ hrefs₁
+          · exact ih₂ hty₂ hrefs₂
 
 theorem typeOf_preserves_valid_refs_or
   {Γ : TypeEnv} (entities : Entities)
   {e₁ e₂ : Expr} {tx : TypedExpr} {c₁ c₂ : Capabilities}
   (hty : typeOf (Expr.or e₁ e₂) c₁ Γ = Except.ok (tx, c₂))
-  (hrefs : entities.ValidRefsFor (Expr.or e₁ e₂)) :
+  (hrefs : entities.ValidRefsFor (Expr.or e₁ e₂))
+  (ih₁ : typeOf_preserves_valid_refs_ih Γ entities e₁)
+  (ih₂ : typeOf_preserves_valid_refs_ih Γ entities e₂) :
   entities.ValidRefsFor tx.toExpr
 := by
   cases hrefs with | or_valid hrefs₁ hrefs₂ =>
@@ -79,7 +144,7 @@ theorem typeOf_preserves_valid_refs_or
     any_goals contradiction
     · simp only [ok, Except.ok.injEq, Prod.mk.injEq, List.nil_eq] at hty
       simp only [←hty.1, TypedExpr.toExpr]
-      exact typeOf_preserves_valid_refs entities hty₁ hrefs₁
+      exact ih₁ hty₁ hrefs₁
     · cases hty₂ : typeOf e₂ c₁ Γ with
       | error => simp [hty₂] at hty
       | ok r₂ =>
@@ -90,8 +155,8 @@ theorem typeOf_preserves_valid_refs_or
         simp only [ok, Except.ok.injEq, Prod.mk.injEq, List.nil_eq] at hty
         simp only [←hty.1, TypedExpr.toExpr]
         constructor
-        · exact typeOf_preserves_valid_refs entities hty₁ hrefs₁
-        · exact typeOf_preserves_valid_refs entities hty₂ hrefs₂
+        · exact ih₁ hty₁ hrefs₁
+        · exact ih₂ hty₂ hrefs₂
     · cases hty₂ : typeOf e₂ c₁ Γ with
       | error => simp [hty₂] at hty
       | ok r₂ =>
@@ -103,16 +168,96 @@ theorem typeOf_preserves_valid_refs_or
           simp only [ok, Except.ok.injEq, Prod.mk.injEq, List.nil_eq] at hty
           simp only [←hty.1, TypedExpr.toExpr]
           constructor
-          · exact typeOf_preserves_valid_refs entities hty₁ hrefs₁
-          · exact typeOf_preserves_valid_refs entities hty₂ hrefs₂
-termination_by sizeOf e₁ + sizeOf e₂
-decreasing_by all_goals sorry
+          · exact ih₁ hty₁ hrefs₁
+          · exact ih₂ hty₂ hrefs₂
+
+theorem typeOf_preserves_valid_refs_ite
+  {Γ : TypeEnv} (entities : Entities)
+  {e₁ e₂ e₃ : Expr} {tx : TypedExpr} {c₁ c₂ : Capabilities}
+  (hty : typeOf (Expr.ite e₁ e₂ e₃) c₁ Γ = Except.ok (tx, c₂))
+  (hrefs : entities.ValidRefsFor (Expr.ite e₁ e₂ e₃))
+  (ih₁ : typeOf_preserves_valid_refs_ih Γ entities e₁)
+  (ih₂ : typeOf_preserves_valid_refs_ih Γ entities e₂)
+  (ih₃ : typeOf_preserves_valid_refs_ih Γ entities e₃) :
+  entities.ValidRefsFor tx.toExpr
+:= by
+  cases hrefs with | ite_valid hrefs₁ hrefs₂ hrefs₃ =>
+  simp only [typeOf, typeOfIf] at hty
+  cases hty₁ : typeOf e₁ c₁ Γ with
+  | error => simp [hty₁] at hty
+  | ok r₁ =>
+    have ⟨tx₁, c₃⟩ := r₁
+    simp only [hty₁, List.empty_eq, Except.bind_ok] at hty
+    split at hty
+    any_goals contradiction
+    · cases hty₂ : typeOf e₂ (c₁ ∪ c₃) Γ with
+      | error => simp [hty₂] at hty
+      | ok r₂ =>
+        have ⟨tx₂, c₄⟩ := r₂
+        simp only [hty₂, ok, Except.bind_ok, Except.ok.injEq, Prod.mk.injEq] at hty
+        simp only [←hty.1, TypedExpr.toExpr]
+        constructor
+        · exact ih₁ hty₁ hrefs₁
+        · exact ih₂ hty₂ hrefs₂
+        · exact ih₂ hty₂ hrefs₂
+    · cases hty₃ : typeOf e₃ c₁ Γ with
+      | error => simp [hty₃] at hty
+      | ok r₃ =>
+        have ⟨tx₃, c₄⟩ := r₃
+        simp only [hty₃, ok, Except.bind_ok, Except.ok.injEq, Prod.mk.injEq] at hty
+        simp only [←hty.1, TypedExpr.toExpr]
+        constructor
+        · exact ih₁ hty₁ hrefs₁
+        · exact ih₃ hty₃ hrefs₃
+        · exact ih₃ hty₃ hrefs₃
+    · cases hty₂ : typeOf e₂ (c₁ ∪ c₃) Γ with
+      | error => simp [hty₂] at hty
+      | ok r₂ =>
+      cases hty₃ : typeOf e₃ c₁ Γ with
+      | error => simp [hty₂, hty₃] at hty
+      | ok r₃ =>
+      have ⟨tx₂, c₄⟩ := r₂
+      have ⟨tx₃, c₅⟩ := r₃
+      simp only [hty₂, hty₃, ok, Except.bind_ok, Except.ok.injEq, Prod.mk.injEq] at hty
+      split at hty
+      · simp only [Except.ok.injEq, Prod.mk.injEq] at hty
+        simp only [←hty.1, TypedExpr.toExpr]
+        constructor
+        · exact ih₁ hty₁ hrefs₁
+        · exact ih₂ hty₂ hrefs₂
+        · exact ih₃ hty₃ hrefs₃
+      · contradiction
+
+theorem typeOf_preserves_valid_refs_unaryApp
+  {Γ : TypeEnv} (entities : Entities)
+  {op : UnaryOp} {e : Expr} {tx : TypedExpr} {c₁ c₂ : Capabilities}
+  (hty : typeOf (Expr.unaryApp op e) c₁ Γ = Except.ok (tx, c₂))
+  (hrefs : entities.ValidRefsFor (Expr.unaryApp op e))
+  (ih : typeOf_preserves_valid_refs_ih Γ entities e) :
+  entities.ValidRefsFor tx.toExpr
+:= by
+  simp only [typeOf, typeOfUnaryApp] at hty
+  cases hrefs with | unaryApp_valid hrefs =>
+  cases hty₁ : typeOf e c₁ Γ with
+  | error => simp [hty₁] at hty
+  | ok r₁ =>
+    have ⟨tx₁, c₃⟩ := r₁
+    simp only [hty₁, List.empty_eq, Except.bind_ok] at hty
+    split at hty
+    any_goals contradiction
+    all_goals
+      simp only [ok, Function.comp_apply, Except.ok.injEq, Prod.mk.injEq, List.nil_eq] at hty
+      simp only [←hty.1, TypedExpr.toExpr]
+      constructor
+      exact ih hty₁ hrefs
 
 theorem typeOf_preserves_valid_refs_binaryApp
   {Γ : TypeEnv} (entities : Entities)
   {op : BinaryOp} {e₁ e₂ : Expr} {tx : TypedExpr} {c₁ c₂ : Capabilities}
   (hty : typeOf (Expr.binaryApp op e₁ e₂) c₁ Γ = Except.ok (tx, c₂))
-  (hrefs : entities.ValidRefsFor (Expr.binaryApp op e₁ e₂)) :
+  (hrefs : entities.ValidRefsFor (Expr.binaryApp op e₁ e₂))
+  (ih₁ : typeOf_preserves_valid_refs_ih Γ entities e₁)
+  (ih₂ : typeOf_preserves_valid_refs_ih Γ entities e₂) :
   entities.ValidRefsFor tx.toExpr
 := by
   simp only [typeOf, typeOfBinaryApp] at hty
@@ -132,8 +277,8 @@ theorem typeOf_preserves_valid_refs_binaryApp
       simp only [ok, Function.comp_apply, Except.ok.injEq, Prod.mk.injEq, List.nil_eq] at hty
       simp only [←hty.1, TypedExpr.toExpr]
       constructor
-      exact typeOf_preserves_valid_refs entities hty₁ hrefs₁
-      exact typeOf_preserves_valid_refs entities hty₂ hrefs₂
+      exact ih₁ hty₁ hrefs₁
+      exact ih₂ hty₂ hrefs₂
     any_goals
       simp only [bind, Except.bind] at hty
       split at hty
@@ -142,8 +287,8 @@ theorem typeOf_preserves_valid_refs_binaryApp
         simp only [ok, Function.comp_apply, Except.ok.injEq, Prod.mk.injEq, List.nil_eq] at hty
         simp only [←hty.1, TypedExpr.toExpr]
         constructor
-        exact typeOf_preserves_valid_refs entities hty₁ hrefs₁
-        exact typeOf_preserves_valid_refs entities hty₂ hrefs₂
+        exact ih₁ hty₁ hrefs₁
+        exact ih₂ hty₂ hrefs₂
     · simp only [typeOfEq] at hty
       split at hty
       · split at hty
@@ -155,8 +300,8 @@ theorem typeOf_preserves_valid_refs_binaryApp
           ] at hty
           simp only [←hty.1, TypedExpr.toExpr]
           constructor
-          exact typeOf_preserves_valid_refs entities hty₁ hrefs₁
-          exact typeOf_preserves_valid_refs entities hty₂ hrefs₂
+          exact ih₁ hty₁ hrefs₁
+          exact ih₂ hty₂ hrefs₂
       · split at hty
         · simp only [
             ok, List.empty_eq, Function.comp_apply,
@@ -165,8 +310,8 @@ theorem typeOf_preserves_valid_refs_binaryApp
           ] at hty
           simp only [←hty.1, TypedExpr.toExpr]
           constructor
-          exact typeOf_preserves_valid_refs entities hty₁ hrefs₁
-          exact typeOf_preserves_valid_refs entities hty₂ hrefs₂
+          exact ih₁ hty₁ hrefs₁
+          exact ih₂ hty₂ hrefs₂
         · split at hty
           · simp only [
               ok, List.empty_eq, Function.comp_apply,
@@ -175,17 +320,127 @@ theorem typeOf_preserves_valid_refs_binaryApp
             ] at hty
             simp only [←hty.1, TypedExpr.toExpr]
             constructor
-            exact typeOf_preserves_valid_refs entities hty₁ hrefs₁
-            exact typeOf_preserves_valid_refs entities hty₂ hrefs₂
+            exact ih₁ hty₁ hrefs₁
+            exact ih₂ hty₂ hrefs₂
           · contradiction
-termination_by sizeOf e₁ + sizeOf e₂
-decreasing_by all_goals sorry
+
+theorem typeOf_preserves_valid_refs_getAttr
+  {Γ : TypeEnv} (entities : Entities)
+  {e : Expr} {attr : Attr} {tx : TypedExpr} {c₁ c₂ : Capabilities}
+  (hty : typeOf (Expr.getAttr e attr) c₁ Γ = Except.ok (tx, c₂))
+  (hrefs : entities.ValidRefsFor (Expr.getAttr e attr))
+  (ih : typeOf_preserves_valid_refs_ih Γ entities e) :
+  entities.ValidRefsFor tx.toExpr
+:= by
+  simp only [typeOf, typeOfGetAttr] at hty
+  cases hrefs with | getAttr_valid hrefs =>
+  cases hty₁ : typeOf e c₁ Γ with
+  | error => simp [hty₁] at hty
+  | ok r₁ =>
+    have ⟨tx₁, c₃⟩ := r₁
+    simp only [hty₁, List.empty_eq, Except.bind_ok] at hty
+    split at hty
+    any_goals contradiction
+    · simp only [bind, Except.bind] at hty
+      split at hty
+      contradiction
+      simp only [ok, Function.comp_apply, Except.ok.injEq, Prod.mk.injEq, List.nil_eq] at hty
+      simp only [←hty.1, TypedExpr.toExpr]
+      constructor
+      exact ih hty₁ hrefs
+    · simp only [bind, Except.bind] at hty
+      split at hty
+      · split at hty
+        contradiction
+        simp only [ok, Function.comp_apply, Except.ok.injEq, Prod.mk.injEq, List.nil_eq] at hty
+        simp only [←hty.1, TypedExpr.toExpr]
+        constructor
+        exact ih hty₁ hrefs
+      · contradiction
+
+theorem typeOf_preserves_valid_refs_hasAttr
+  {Γ : TypeEnv} (entities : Entities)
+  {e : Expr} {attr : Attr} {tx : TypedExpr} {c₁ c₂ : Capabilities}
+  (hty : typeOf (Expr.hasAttr e attr) c₁ Γ = Except.ok (tx, c₂))
+  (hrefs : entities.ValidRefsFor (Expr.hasAttr e attr))
+  (ih : typeOf_preserves_valid_refs_ih Γ entities e) :
+  entities.ValidRefsFor tx.toExpr
+:= by
+  simp only [typeOf, typeOfHasAttr] at hty
+  cases hrefs with | hasAttr_valid hrefs =>
+  cases hty₁ : typeOf e c₁ Γ with
+  | error => simp [hty₁] at hty
+  | ok r₁ =>
+    have ⟨tx₁, c₃⟩ := r₁
+    simp only [hty₁, List.empty_eq, Except.bind_ok] at hty
+    split at hty
+    any_goals contradiction
+    · simp only [bind, Except.bind] at hty
+      split at hty
+      contradiction
+      simp only [ok, Function.comp_apply, Except.ok.injEq, Prod.mk.injEq, List.nil_eq] at hty
+      simp only [←hty.1, TypedExpr.toExpr]
+      constructor
+      exact ih hty₁ hrefs
+    · simp only [bind, Except.bind] at hty
+      split at hty
+      · split at hty
+        contradiction
+        simp only [ok, Function.comp_apply, Except.ok.injEq, Prod.mk.injEq, List.nil_eq] at hty
+        simp only [←hty.1, TypedExpr.toExpr]
+        constructor
+        exact ih hty₁ hrefs
+      · split at hty
+        · simp only [ok, Function.comp_apply, Except.ok.injEq, Prod.mk.injEq, List.nil_eq] at hty
+          simp only [←hty.1, TypedExpr.toExpr]
+          constructor
+          exact ih hty₁ hrefs
+        · contradiction
+
+theorem typeOf_preserves_valid_refs_set
+  {Γ : TypeEnv} (entities : Entities)
+  {s : List Expr} {tx : TypedExpr} {c₁ c₂ : Capabilities}
+  (hty : typeOf (Expr.set s) c₁ Γ = Except.ok (tx, c₂))
+  (hrefs : entities.ValidRefsFor (Expr.set s))
+  (ih_xs : ∀ x ∈ s, typeOf_preserves_valid_refs_ih Γ entities x) :
+  entities.ValidRefsFor tx.toExpr
+:= by
+  simp only [typeOf, typeOfSet] at hty
+  cases hrefs with | set_valid hrefs =>
+  simp only [bind, Except.bind] at hty
+  split at hty
+  contradiction
+  rename_i s' hs'
+  split at hty
+  contradiction
+  rename_i hd tl
+  split at hty
+  · rename_i ty _
+    simp only [ok, List.empty_eq, Except.ok.injEq, Prod.mk.injEq, List.nil_eq] at hty
+    simp only [←hty.1, TypedExpr.toExpr]
+    constructor
+    intros x' hmem_x'
+    simp only [List.map₁_eq_map] at hmem_x'
+    have ⟨tx', hmem_tx', htx'⟩ := List.mem_map.mp hmem_x'
+    simp only [List.mapM₁_eq_mapM (λ x => justType (typeOf x c₁ Γ)) _] at hs'
+    have ⟨x, hmem_x, hx⟩ := List.mapM_ok_implies_all_from_ok hs' tx' hmem_tx'
+    simp only [justType] at hx
+    cases htyₓ : typeOf x c₁ Γ with
+    | error => simp [htyₓ, Except.map] at hx
+    | ok r =>
+      have ⟨tx, c₄⟩ := r
+      simp only [htyₓ, Except.map, Except.ok.injEq] at hx
+      simp only [←htx', ←hx]
+      specialize hrefs x hmem_x
+      exact ih_xs x hmem_x htyₓ hrefs
+  · contradiction
 
 theorem typeOf_preserves_valid_refs_call
   {Γ : TypeEnv} (entities : Entities)
   {xfn : ExtFun} {args : List Expr} {tx : TypedExpr} {c₁ c₂ : Capabilities}
   (hty : typeOf (Expr.call xfn args) c₁ Γ = Except.ok (tx, c₂))
-  (hrefs : entities.ValidRefsFor (Expr.call xfn args)) :
+  (hrefs : entities.ValidRefsFor (Expr.call xfn args))
+  (ih_args : ∀ arg ∈ args, typeOf_preserves_valid_refs_ih Γ entities arg) :
   entities.ValidRefsFor tx.toExpr
 := by
   simp only [typeOf, typeOfCall, bind, Except.bind] at hty
@@ -214,15 +469,14 @@ theorem typeOf_preserves_valid_refs_call
       simp only [htyₓ, Except.map, Except.ok.injEq] at hx
       simp only [←htx', ←hx]
       specialize hrefs x hmem_x
-      exact typeOf_preserves_valid_refs entities htyₓ hrefs
-termination_by sizeOf args
-decreasing_by all_goals sorry
+      exact ih_args x hmem_x htyₓ hrefs
 
 theorem typeOf_preserves_valid_refs_record
   {Γ : TypeEnv} (entities : Entities)
   {rec : List (Attr × Expr)} {tx : TypedExpr} {c₁ c₂ : Capabilities}
   (hty : typeOf (Expr.record rec) c₁ Γ = Except.ok (tx, c₂))
-  (hrefs : entities.ValidRefsFor (Expr.record rec)) :
+  (hrefs : entities.ValidRefsFor (Expr.record rec))
+  (ih_rec : ∀ attr ∈ rec, typeOf_preserves_valid_refs_ih Γ entities attr.snd) :
   entities.ValidRefsFor tx.toExpr
 := by
   simp only [typeOf, bind, Except.bind] at hty
@@ -248,9 +502,7 @@ theorem typeOf_preserves_valid_refs_record
     simp only [Except.map, htyₓ, Except.ok.injEq, Prod.mk.injEq] at hattr'_x
     simp only [←hattr'_x]
     specialize hrefs (attr', x) hmem_attr'_x
-    exact typeOf_preserves_valid_refs entities htyₓ hrefs
-termination_by sizeOf recs
-decreasing_by all_goals sorry
+    exact ih_rec (attr', x) hmem_attr'_x htyₓ hrefs
 
 /--
 `typeOf` preserves `Entities.ValidRefsFor`.
@@ -270,207 +522,59 @@ theorem typeOf_preserves_valid_refs
   entities.ValidRefsFor tx.toExpr
 := by
   cases expr with
-  | lit p =>
-    simp only [typeOf, typeOfLit] at hty
-    cases p with
-    | bool | int | string =>
-      split at hty
-      any_goals contradiction
-      all_goals
-        simp only [
-          ok, List.empty_eq,
-          Function.comp_apply,
-          Except.ok.injEq,
-          Prod.mk.injEq,
-          List.nil_eq,
-        ] at hty
-        simp only [←hty.1, TypedExpr.toExpr]
-        repeat constructor
-    | entityUID uid =>
-      split at hty
-      any_goals contradiction
-      all_goals
-        split at hty
-        · simp only [
-            ok, List.empty_eq,
-            Function.comp_apply,
-            Except.ok.injEq,
-            Prod.mk.injEq,
-            List.nil_eq,
-          ] at hty
-          simp only [←hty.1, TypedExpr.toExpr]
-          constructor
-          cases hrefs
-          assumption
-        · contradiction
-  | var v =>
-    simp only [typeOf, typeOfVar] at hty
-    split at hty
-    all_goals
-      simp only [
-        ok, List.empty_eq, Function.comp_apply,
-        Except.ok.injEq, Prod.mk.injEq,
-        List.nil_eq,
-      ] at hty
-      simp only [←hty.1, TypedExpr.toExpr]
-      constructor
-  | and e₁ e₂ => exact typeOf_preserves_valid_refs_and entities hty hrefs
-  | or e₁ e₂ => exact typeOf_preserves_valid_refs_or entities hty hrefs
+  | lit p => exact typeOf_preserves_valid_refs_lit entities hty hrefs
+  | var v => exact typeOf_preserves_valid_refs_var entities hty hrefs
+  | and e₁ e₂ =>
+    apply typeOf_preserves_valid_refs_and entities hty hrefs
+    · intros tx c c'; apply typeOf_preserves_valid_refs
+    · intros tx c c'; apply typeOf_preserves_valid_refs
+  | or e₁ e₂ =>
+    apply typeOf_preserves_valid_refs_or entities hty hrefs
+    · intros tx c c'; apply typeOf_preserves_valid_refs
+    · intros tx c c'; apply typeOf_preserves_valid_refs
   | ite e₁ e₂ e₃ =>
-    cases hrefs with | ite_valid hrefs₁ hrefs₂ hrefs₃ =>
-    simp only [typeOf, typeOfIf] at hty
-    cases hty₁ : typeOf e₁ c₁ Γ with
-    | error => simp [hty₁] at hty
-    | ok r₁ =>
-      have ⟨tx₁, c₃⟩ := r₁
-      simp only [hty₁, List.empty_eq, Except.bind_ok] at hty
-      split at hty
-      any_goals contradiction
-      · cases hty₂ : typeOf e₂ (c₁ ∪ c₃) Γ with
-        | error => simp [hty₂] at hty
-        | ok r₂ =>
-          have ⟨tx₂, c₄⟩ := r₂
-          simp only [hty₂, ok, Except.bind_ok, Except.ok.injEq, Prod.mk.injEq] at hty
-          simp only [←hty.1, TypedExpr.toExpr]
-          constructor
-          · exact typeOf_preserves_valid_refs entities hty₁ hrefs₁
-          · exact typeOf_preserves_valid_refs entities hty₂ hrefs₂
-          · exact typeOf_preserves_valid_refs entities hty₂ hrefs₂
-      · cases hty₃ : typeOf e₃ c₁ Γ with
-        | error => simp [hty₃] at hty
-        | ok r₃ =>
-          have ⟨tx₃, c₄⟩ := r₃
-          simp only [hty₃, ok, Except.bind_ok, Except.ok.injEq, Prod.mk.injEq] at hty
-          simp only [←hty.1, TypedExpr.toExpr]
-          constructor
-          · exact typeOf_preserves_valid_refs entities hty₁ hrefs₁
-          · exact typeOf_preserves_valid_refs entities hty₃ hrefs₃
-          · exact typeOf_preserves_valid_refs entities hty₃ hrefs₃
-      · cases hty₂ : typeOf e₂ (c₁ ∪ c₃) Γ with
-        | error => simp [hty₂] at hty
-        | ok r₂ =>
-        cases hty₃ : typeOf e₃ c₁ Γ with
-        | error => simp [hty₂, hty₃] at hty
-        | ok r₃ =>
-        have ⟨tx₂, c₄⟩ := r₂
-        have ⟨tx₃, c₅⟩ := r₃
-        simp only [hty₂, hty₃, ok, Except.bind_ok, Except.ok.injEq, Prod.mk.injEq] at hty
-        split at hty
-        · simp only [Except.ok.injEq, Prod.mk.injEq] at hty
-          simp only [←hty.1, TypedExpr.toExpr]
-          constructor
-          · exact typeOf_preserves_valid_refs entities hty₁ hrefs₁
-          · exact typeOf_preserves_valid_refs entities hty₂ hrefs₂
-          · exact typeOf_preserves_valid_refs entities hty₃ hrefs₃
-        · contradiction
+    apply typeOf_preserves_valid_refs_ite entities hty hrefs
+    · intros tx c c'; apply typeOf_preserves_valid_refs
+    · intros tx c c'; apply typeOf_preserves_valid_refs
+    · intros tx c c'; apply typeOf_preserves_valid_refs
   | unaryApp _ e =>
-    simp only [typeOf, typeOfUnaryApp] at hty
-    cases hrefs with | unaryApp_valid hrefs =>
-    cases hty₁ : typeOf e c₁ Γ with
-    | error => simp [hty₁] at hty
-    | ok r₁ =>
-      have ⟨tx₁, c₃⟩ := r₁
-      simp only [hty₁, List.empty_eq, Except.bind_ok] at hty
-      split at hty
-      any_goals contradiction
-      all_goals
-        simp only [ok, Function.comp_apply, Except.ok.injEq, Prod.mk.injEq, List.nil_eq] at hty
-        simp only [←hty.1, TypedExpr.toExpr]
-        constructor
-        exact typeOf_preserves_valid_refs entities hty₁ hrefs
-  | binaryApp _ e₁ e₂ => exact typeOf_preserves_valid_refs_binaryApp entities hty hrefs
+    apply typeOf_preserves_valid_refs_unaryApp entities hty hrefs
+    intros tx c c'; apply typeOf_preserves_valid_refs
+  | binaryApp _ e₁ e₂ =>
+    apply typeOf_preserves_valid_refs_binaryApp entities hty hrefs
+    · intros tx c c'; apply typeOf_preserves_valid_refs
+    · intros tx c c'; apply typeOf_preserves_valid_refs
   | getAttr e _ =>
-    simp only [typeOf, typeOfGetAttr] at hty
-    cases hrefs with | getAttr_valid hrefs =>
-    cases hty₁ : typeOf e c₁ Γ with
-    | error => simp [hty₁] at hty
-    | ok r₁ =>
-      have ⟨tx₁, c₃⟩ := r₁
-      simp only [hty₁, List.empty_eq, Except.bind_ok] at hty
-      split at hty
-      any_goals contradiction
-      · simp only [bind, Except.bind] at hty
-        split at hty
-        contradiction
-        simp only [ok, Function.comp_apply, Except.ok.injEq, Prod.mk.injEq, List.nil_eq] at hty
-        simp only [←hty.1, TypedExpr.toExpr]
-        constructor
-        exact typeOf_preserves_valid_refs entities hty₁ hrefs
-      · simp only [bind, Except.bind] at hty
-        split at hty
-        · split at hty
-          contradiction
-          simp only [ok, Function.comp_apply, Except.ok.injEq, Prod.mk.injEq, List.nil_eq] at hty
-          simp only [←hty.1, TypedExpr.toExpr]
-          constructor
-          exact typeOf_preserves_valid_refs entities hty₁ hrefs
-        · contradiction
+    apply typeOf_preserves_valid_refs_getAttr entities hty hrefs
+    intros tx c c'; apply typeOf_preserves_valid_refs
   | hasAttr e _ =>
-    simp only [typeOf, typeOfHasAttr] at hty
-    cases hrefs with | hasAttr_valid hrefs =>
-    cases hty₁ : typeOf e c₁ Γ with
-    | error => simp [hty₁] at hty
-    | ok r₁ =>
-      have ⟨tx₁, c₃⟩ := r₁
-      simp only [hty₁, List.empty_eq, Except.bind_ok] at hty
-      split at hty
-      any_goals contradiction
-      · simp only [bind, Except.bind] at hty
-        split at hty
-        contradiction
-        simp only [ok, Function.comp_apply, Except.ok.injEq, Prod.mk.injEq, List.nil_eq] at hty
-        simp only [←hty.1, TypedExpr.toExpr]
-        constructor
-        exact typeOf_preserves_valid_refs entities hty₁ hrefs
-      · simp only [bind, Except.bind] at hty
-        split at hty
-        · split at hty
-          contradiction
-          simp only [ok, Function.comp_apply, Except.ok.injEq, Prod.mk.injEq, List.nil_eq] at hty
-          simp only [←hty.1, TypedExpr.toExpr]
-          constructor
-          exact typeOf_preserves_valid_refs entities hty₁ hrefs
-        · split at hty
-          · simp only [ok, Function.comp_apply, Except.ok.injEq, Prod.mk.injEq, List.nil_eq] at hty
-            simp only [←hty.1, TypedExpr.toExpr]
-            constructor
-            exact typeOf_preserves_valid_refs entities hty₁ hrefs
-          · contradiction
+    apply typeOf_preserves_valid_refs_hasAttr entities hty hrefs
+    intros tx c c'; apply typeOf_preserves_valid_refs
   | set s =>
-    simp only [typeOf, typeOfSet] at hty
-    cases hrefs with | set_valid hrefs =>
-    simp only [bind, Except.bind] at hty
-    split at hty
-    contradiction
-    rename_i s' hs'
-    split at hty
-    contradiction
-    rename_i hd tl
-    split at hty
-    · rename_i ty _
-      simp only [ok, List.empty_eq, Except.ok.injEq, Prod.mk.injEq, List.nil_eq] at hty
-      simp only [←hty.1, TypedExpr.toExpr]
-      constructor
-      intros x' hmem_x'
-      simp only [List.map₁_eq_map] at hmem_x'
-      have ⟨tx', hmem_tx', htx'⟩ := List.mem_map.mp hmem_x'
-      simp only [List.mapM₁_eq_mapM (λ x => justType (typeOf x c₁ Γ)) _] at hs'
-      have ⟨x, hmem_x, hx⟩ := List.mapM_ok_implies_all_from_ok hs' tx' hmem_tx'
-      simp only [justType] at hx
-      cases htyₓ : typeOf x c₁ Γ with
-      | error => simp [htyₓ, Except.map] at hx
-      | ok r =>
-        have ⟨tx, c₄⟩ := r
-        simp only [htyₓ, Except.map, Except.ok.injEq] at hx
-        simp only [←htx', ←hx]
-        specialize hrefs x hmem_x
-        exact typeOf_preserves_valid_refs entities htyₓ hrefs
-    · contradiction
-  | call _ args => exact typeOf_preserves_valid_refs_call entities hty hrefs
-  | record rec => exact typeOf_preserves_valid_refs_record entities hty hrefs
+    apply typeOf_preserves_valid_refs_set entities hty hrefs
+    intros x hmem_x tx c c'
+    apply typeOf_preserves_valid_refs
+  | call _ args =>
+    apply typeOf_preserves_valid_refs_call entities hty hrefs
+    intros arg hmem_arg tx c c'
+    apply typeOf_preserves_valid_refs
+  | record rec =>
+    apply typeOf_preserves_valid_refs_record entities hty hrefs
+    intros attr hmem_attr tx c c'
+    apply typeOf_preserves_valid_refs
 termination_by sizeOf expr
-decreasing_by all_goals sorry
-
-end
+decreasing_by
+  any_goals simp [*]; omega
+  · simp [*]
+    have := List.sizeOf_lt_of_mem hmem_x
+    omega
+  · simp [*]
+    have := List.sizeOf_lt_of_mem hmem_attr
+    cases attr
+    simp at this ⊢
+    omega
+  · simp [*]
+    have := List.sizeOf_lt_of_mem hmem_arg
+    omega
 
 end Cedar.Thm
